thys/Monitor_Code.thy
@@ -20,11 +20,11 @@ lemma image_these: "f ` Option.these X = Option.these (map_option f ` X)"
   by (force simp: in_these_eq Bex_def image_iff map_option_case split: option.splits)
 
 lemma meval_MPred: "meval n t db (MPred e ts) = ([Option.these
-  ((map_option (\<lambda>f. tabulate f 0 n) o match ts) ` (\<Union>(e', x)\<in>db. if e = e' then {x} else {}))], MPred e ts)"
+  ((map_option (\<lambda>f. Table.tabulate f 0 n) o match ts) ` (\<Union>(e', x)\<in>db. if e = e' then {x} else {}))], MPred e ts)"
   unfolding meval.simps image_these image_image o_def ..
 
 lemma meval_MPred': "meval n t db (MPred e ts) = ([Option.these
-  (\<Union>(e', x)\<in>db. if e = e' then {map_option (\<lambda>f. tabulate f 0 n) (match ts x)} else {})], MPred e ts)"
+  (\<Union>(e', x)\<in>db. if e = e' then {map_option (\<lambda>f. Table.tabulate f 0 n) (match ts x)} else {})], MPred e ts)"
   unfolding meval_MPred image_UN split_beta if_distrib[of "image _"] image_insert image_empty o_apply
   ..
 
@@ -32,7 +32,7 @@ lemma these_UNION: "Option.these (UNION A B) = UNION A (Option.these o B)"
   by (auto simp: Option.these_def)
 
 lemma meval_MPred'': "meval n t db (MPred e ts) = ([
-  (\<Union>(e', x)\<in>db. if e = e' then set_option (map_option (\<lambda>f. tabulate f 0 n) (match ts x)) else {})], MPred e ts)"
+  (\<Union>(e', x)\<in>db. if e = e' then set_option (map_option (\<lambda>f. Table.tabulate f 0 n) (match ts x)) else {})], MPred e ts)"
   unfolding meval_MPred' these_UNION o_def prod.case_distrib[of Option.these]
   by (auto simp: Option.these_def map_option_case image_iff split: if_splits option.splits)
 
